Updated cps.v and eval.v to correspond to the new syntax and semantics. Fixed most of the L6 related files including the closure conversion and hoisting transformations and proofs.

certicoq/theories/L6_PCPS/ctx.v
@@ -3,24 +3,26 @@ Require Import cps.
 
 Import ListNotations.
 
+(** Expression evaluation contexts *)
 Inductive exp_ctx : Type :=
 | Hole_c : exp_ctx
-| Econstr_c : var -> type -> tag -> list var -> exp_ctx -> exp_ctx
-| Eproj_c  : var -> type -> N -> var -> exp_ctx -> exp_ctx
-| Eprim_c : var -> type -> prim -> list var -> exp_ctx -> exp_ctx   
-| Ecase_c : var -> list (tag * exp) -> tag ->
-            exp_ctx -> list (tag * exp) -> exp_ctx  
+| Econstr_c : var -> cTag -> list var -> exp_ctx -> exp_ctx
+| Eproj_c  : var -> cTag -> N -> var -> exp_ctx -> exp_ctx
+| Eprim_c : var -> prim -> list var -> exp_ctx -> exp_ctx   
+| Ecase_c : var -> list (cTag * exp) -> cTag ->
+            exp_ctx -> list (cTag * exp) -> exp_ctx  
 | Efun1_c : fundefs -> exp_ctx -> exp_ctx
 | Efun2_c : fundefs_ctx -> exp -> exp_ctx
 with fundefs_ctx :=
-     | Fcons1_c:  var -> type -> list var -> exp_ctx -> fundefs -> fundefs_ctx
-     | Fcons2_c:  var -> type -> list var -> exp -> fundefs_ctx -> fundefs_ctx.
+     | Fcons1_c:  var -> cTag -> list var -> exp_ctx -> fundefs -> fundefs_ctx
+     | Fcons2_c:  var -> cTag -> list var -> exp -> fundefs_ctx -> fundefs_ctx.
 
+(** Evaluation context application - Relational definition *)
 Inductive app_ctx: exp_ctx -> exp -> exp -> Prop :=
 | Hole_ac: forall e, app_ctx Hole_c e e
-| Constr_ac : forall x t k c ys e ce,
+| Constr_ac : forall x t c ys e ce,
                 app_ctx c e ce ->        
-                app_ctx (Econstr_c x t k ys c) e (Econstr x t k ys ce)
+                app_ctx (Econstr_c x t ys c) e (Econstr x t ys ce)
 | Proj_ac : forall x t n y e c ce, 
               app_ctx c e ce ->        
               app_ctx (Eproj_c x t n y c) e (Eproj x t n y ce)
@@ -28,9 +30,9 @@ Inductive app_ctx: exp_ctx -> exp -> exp -> Prop :=
               app_ctx c e ce ->
               app_ctx (Ecase_c x te t c te') e
                       (Ecase x (te ++ (t, ce) :: te')) 
-| Prim_ac : forall x t f ys e c ce, 
+| Prim_ac : forall x f ys e c ce, 
               app_ctx c e ce ->        
-              app_ctx (Eprim_c x t f ys c) e (Eprim x t f ys ce)
+              app_ctx (Eprim_c x f ys c) e (Eprim x f ys ce)
 | Fun1_ac : forall c e ce fds,
               app_ctx c e ce ->
               app_ctx (Efun1_c fds c) e (Efun fds ce)
@@ -47,14 +49,15 @@ with app_f_ctx : fundefs_ctx -> exp -> fundefs -> Prop :=
 
 Hint Constructors app_ctx app_f_ctx.
 
+(** Evaluation context application - Computational definition *)
 Fixpoint app_ctx_f (c:exp_ctx) (e:exp) : exp :=
   match c with
     | Hole_c => e
-    | Econstr_c x t k ys c => Econstr x t k ys (app_ctx_f c e)
+    | Econstr_c x t ys c => Econstr x t ys (app_ctx_f c e)
     | Eproj_c x t n y c => Eproj x t n y (app_ctx_f c e)
     | Ecase_c x te t c te' =>
       Ecase x (te ++ (t, app_ctx_f c e) :: te')
-    | Eprim_c x t f ys c => Eprim x t f ys (app_ctx_f c e)
+    | Eprim_c x f ys c => Eprim x f ys (app_ctx_f c e)
     | Efun1_c fds c => Efun fds (app_ctx_f c e)
     | Efun2_c cfds e' => Efun (app_f_ctx_f cfds e) e' 
   end
@@ -64,20 +67,21 @@ with app_f_ctx_f (c: fundefs_ctx) (e:exp) : fundefs :=
          | Fcons2_c f t ys e' cfds => Fcons f t ys e' (app_f_ctx_f cfds e)
        end.
 
+(** Composition of evaluation context - Relational definition *)
 Inductive  comp_ctx: exp_ctx -> exp_ctx -> exp_ctx -> Prop :=
 | Hole_cc: forall e, comp_ctx Hole_c e e
-| Constr_cc : forall x t k c ys e ce,
+| Constr_cc : forall x t c ys e ce,
                 comp_ctx c e ce ->
-                comp_ctx (Econstr_c x t k ys c) e (Econstr_c x t k ys ce)
+                comp_ctx (Econstr_c x t ys c) e (Econstr_c x t ys ce)
 | Proj_cc : forall x t n y e c ce,
               comp_ctx c e ce ->
               comp_ctx (Eproj_c x t n y c) e (Eproj_c x t n y ce)
 | Case_cc : forall x te t c te' c' cc,
               comp_ctx c c' cc ->
               comp_ctx (Ecase_c x te t c te') c' (Ecase_c x te t cc te')
-| Prim_cc : forall x t f ys e c ce,
+| Prim_cc : forall x f ys e c ce,
               comp_ctx c e ce ->
-              comp_ctx (Eprim_c x t f ys c) e (Eprim_c x t f ys ce)
+              comp_ctx (Eprim_c x f ys c) e (Eprim_c x f ys ce)
 | Fun1_cc : forall c e ce fds,
               comp_ctx c e ce ->
               comp_ctx (Efun1_c fds c) e (Efun1_c fds ce)
@@ -94,13 +98,14 @@ with comp_f_ctx : fundefs_ctx -> exp_ctx -> fundefs_ctx -> Prop :=
            comp_f_ctx cfds e cfdse ->
            comp_f_ctx (Fcons2_c f t ys e' cfds) e (Fcons2_c f t ys e' cfdse).
 
+(** Composition of evaluation context - Computational definition *)
 Fixpoint comp_ctx_f (c1:exp_ctx) (c2:exp_ctx) : exp_ctx :=
   match c1 with
     | Hole_c => c2
-    | Econstr_c x t k ys c => Econstr_c x t k ys (comp_ctx_f c c2)
+    | Econstr_c x t ys c => Econstr_c x t ys (comp_ctx_f c c2)
     | Eproj_c x t n y c => Eproj_c x t n y (comp_ctx_f c c2)
     | Ecase_c x te t c te' => Ecase_c x te t (comp_ctx_f c c2) te'
-    | Eprim_c x t f ys c => Eprim_c x t f ys (comp_ctx_f c c2)
+    | Eprim_c x f ys c => Eprim_c x f ys (comp_ctx_f c c2)
     | Efun1_c fds c => Efun1_c fds (comp_ctx_f c c2)
     | Efun2_c cfds e' => Efun2_c (comp_f_ctx_f cfds c2) e'
   end
@@ -116,6 +121,7 @@ Notation "c '|[' e ']|' " := (app_ctx_f c e)  (at level 28, no associativity)
                              : ctx_scope.
 Notation "f '<[' e ']>'" := (app_f_ctx_f f e)  (at level 28, no associativity)
                             : ctx_scope.
+Open Scope ctx_scope.
 
 Scheme ctx_exp_mut := Induction for exp_ctx Sort Prop
                       with ctx_fundefs_mut := Induction for fundefs_ctx Sort Prop.
@@ -123,19 +129,19 @@ Scheme ctx_exp_mut := Induction for exp_ctx Sort Prop
 Lemma exp_fundefs_ctx_mutual_ind :
   forall (P : exp_ctx -> Prop) (P0 : fundefs_ctx -> Prop),
     P Hole_c ->
-    (forall (v : var) (t : type) (t0 : tag) (l : list var) (e : exp_ctx),
-       P e -> P (Econstr_c v t t0 l e)) ->
-    (forall (v : var) (t : type) (n : N) (v0 : var) (e : exp_ctx),
+    (forall (v : var) (t : cTag) (l : list var) (e : exp_ctx),
+       P e -> P (Econstr_c v t l e)) ->
+    (forall (v : var) (t : cTag) (n : N) (v0 : var) (e : exp_ctx),
        P e -> P (Eproj_c v t n v0 e)) ->
-    (forall (v : var) (t : type) (p : prim) (l : list var) (e : exp_ctx),
-       P e -> P (Eprim_c v t p l e)) ->
-    (forall (v : var) (l : list (tag * exp)) (t : tag) (e : exp_ctx),
-       P e -> forall l0 : list (tag * exp), P (Ecase_c v l t e l0)) ->
+    (forall (v : var) (p : prim) (l : list var) (e : exp_ctx),
+       P e -> P (Eprim_c v p l e)) ->
+    (forall (v : var) (l : list (cTag * exp)) (t : cTag) (e : exp_ctx),
+       P e -> forall l0 : list (cTag * exp), P (Ecase_c v l t e l0)) ->
     (forall (f4 : fundefs) (e : exp_ctx), P e -> P (Efun1_c f4 e)) ->
     (forall f5 : fundefs_ctx, P0 f5 -> forall e : exp, P (Efun2_c f5 e)) ->
-    (forall (v : var) (t : type) (l : list var) (e : exp_ctx),
+    (forall (v : var) (t : fTag) (l : list var) (e : exp_ctx),
        P e -> forall f6 : fundefs, P0 (Fcons1_c v t l e f6)) ->
-    (forall (v : var) (t : type) (l : list var) 
+    (forall (v : var) (t : fTag) (l : list var) 
             (e : exp) (f7 : fundefs_ctx), P0 f7 -> P0 (Fcons2_c v t l e f7)) ->
     (forall e : exp_ctx, P e) /\ (forall f : fundefs_ctx, P0 f).
 Proof.
@@ -144,46 +150,114 @@ Proof.
   apply (ctx_fundefs_mut P P0); assumption.
 Qed.
 
-(** name the induction hypotheses only *)
+(** Name the induction hypotheses only *)
 Ltac exp_fundefs_ctx_induction IH1 IH2 :=
   apply exp_fundefs_ctx_mutual_ind;
-  [ | intros ? ? ? ? ? IH1 
+  [ | intros ? ? ? ? IH1 
     | intros ? ? ? ? ? IH1
-    | intros ? ? ? ? ? IH1
+    | intros ? ? ? ? IH1
     | intros ? ? ? ? IH1
     | intros ? ? IH1
     | intros ? IH2 ?
     | intros ? ? ? ? IH1 ?
     | intros ? ? ? ? ? IH2 ].
 
-(** alternative definition of subterms relation *)
+(** Alternative definition of subterm relation *)
 Definition subterm_e' (e':exp) (e:exp): Prop :=
   exists c, Hole_c <> c /\ app_ctx c e' e.
 
 Definition subterm_or_eq' (e':exp) (e:exp) : Prop :=
   exists c, app_ctx c e' e.
 
-(** theorems about app and comp *)
-Lemma app_ctx_f_correct:
+(** Theorems about context application and composition *)
+Lemma app_ctx_f_correct_mut:
+  (forall c e e',
+     c |[ e ]|  = e' <-> app_ctx c e e') /\
+  (forall cf B B',
+     cf <[ B ]> = B' <-> app_f_ctx cf B B').
+Proof. 
+  exp_fundefs_ctx_induction IHe IHf; simpl; intros; split; intros H';
+  first
+    [ inversion H'; subst; constructor;
+      eapply IHe; congruence
+    | inversion H'; subst; repeat f_equal; eapply IHe;
+      eassumption
+    | inversion H'; subst; constructor;
+      eapply IHf; congruence
+    | inversion H'; subst; repeat f_equal; eapply IHf ];
+  inversion H'; subst; eassumption.
+Qed.
+
+Corollary app_ctx_f_correct :
   forall c e e',
-    app_ctx_f c e  = e' <-> app_ctx c e e'
-    with app_f_ctx_f_correct:
-           forall cf e e',
-             app_f_ctx_f cf e = e' <-> app_f_ctx cf e e'.
-Admitted.
+    c |[ e ]|  = e' <-> app_ctx c e e'.
+Proof.
+  now apply app_ctx_f_correct_mut.
+Qed.
 
-Lemma comp_ctx_f_correct:
+Corollary app_f_ctx_f_correct :
+  forall cf B B',
+    cf <[ B ]> = B' <-> app_f_ctx cf B B'.
+Proof.
+  now apply app_ctx_f_correct_mut.
+Qed.
+
+Lemma comp_ctx_f_correct_mut:
+  (forall c c' cc',
+     comp_ctx_f c c'  = cc' <-> comp_ctx c c' cc') /\
+  (forall cf cf' ccf',
+     comp_f_ctx_f cf cf' = ccf' <-> comp_f_ctx cf cf' ccf').
+Proof. 
+  exp_fundefs_ctx_induction IHe IHf; simpl; intros; split; intros H';
+  first
+    [ inversion H'; subst; constructor;
+      eapply IHe; congruence
+    | inversion H'; subst; repeat f_equal; eapply IHe;
+      eassumption
+    | inversion H'; subst; constructor;
+      eapply IHf; congruence
+    | inversion H'; subst; repeat f_equal; eapply IHf ];
+  inversion H'; subst; eassumption.
+Qed.
+
+Corollary comp_ctx_f_correct :
   forall c c' cc',
-    comp_ctx_f c c'  = cc' <-> comp_ctx c c' cc'
-    with comp_f_ctx_f_correct:
-           forall cf cf' ccf',
-             comp_f_ctx_f cf cf' = ccf' <-> comp_f_ctx cf cf' ccf'.
-Admitted.
+    comp_ctx_f c c'  = cc' <-> comp_ctx c c' cc'.
+Proof.
+  now apply comp_ctx_f_correct_mut.
+Qed.
 
-Lemma app_ctx_f_fuse :
+Corollary comp_f_ctx_f_correct :
+  forall cf cf' ccf',
+   comp_f_ctx_f cf cf' = ccf' <-> comp_f_ctx cf cf' ccf'.
+Proof.
+  now apply comp_ctx_f_correct_mut.
+Qed.
+
+Lemma app_ctx_f_fuse_mut :
+  (forall c c' e,
+     c |[ c' |[ e ]| ]| = (comp_ctx_f c c') |[ e ]|) /\
+  (forall cf c e,
+     cf <[ c |[ e ]| ]> = (comp_f_ctx_f cf c) <[ e ]>).
+Proof.
+  exp_fundefs_ctx_induction IHe IHf; simpl; intros;
+  try (rewrite IHe; reflexivity); try (rewrite IHf; reflexivity).
+  reflexivity.
+Qed.
+
+Corollary app_ctx_f_fuse :
   forall c c' e,
-    app_ctx_f c (app_ctx_f c' e) = app_ctx_f (comp_ctx_f c c') e.
-Admitted. 
+    c |[ c' |[ e ]| ]| = (comp_ctx_f c c') |[ e ]|.
+Proof.
+  now apply app_ctx_f_fuse_mut.
+Qed.
+
+Corollary app_f_ctx_f_fuse :
+  forall cf c e,
+    cf <[ c |[ e ]| ]> = (comp_f_ctx_f cf c) <[ e ]>.
+Proof.
+  now apply app_ctx_f_fuse_mut.
+Qed.
 
 Lemma app_ctx_fuse:
   forall (c c' : exp_ctx) (e1 e2 e3 : exp),
